examples/unit-tests/acls2.fst
@@ -99,4 +99,3 @@ let test_acls f =
   (* let _ = read f in       (\* not ok any more *\) *)
   ()
 
-
