examples/unit-tests/format.fst
@@ -10,17 +10,7 @@
    Unless required by applicable law or agreed to in writing, software
    distributed under the License is distributed on an "AS IS" BASIS,
    WITHOUT WARRANTIES OR CONDITIONS OF ANY KIND, either express or implied.
-   See the License for the specific language governing permissions and
-   limitations under the License.
-*)
-
-module Format
-open Prims.PURE
-open String
-open Array
-
-type message = seq byte
-type msg (l:nat) = m:message{length m==l}
+   See the License for the :nat) = m:message{length m==l}
 
 (* ----- two lemmas on array append *) 
 
