examples/unit-tests/hybrid2.fst
@@ -10,7 +10,9 @@ let ciphersize = PKE.ciphersize + SymEnc.ciphersize
  
 let enc t = 
   let k = SymEnc.keygen true in 
-  append (PKE.encrypt pk k) (SymEnc.encrypt k t)
+  append 
+    (PKE.encrypt pk k) 
+    (SymEnc.encrypt k t)
 
 let dec c =
   let c0,c1 = split c PKE.ciphersize in 
