examples/unit-tests/mac2.fst
@@ -47,14 +47,10 @@ let sha1verify k txt tag = (sha1 k txt = tag)
 opaque type key_prop : key -> text -> Type
 type pkey (p:(text -> Type)) = k:key{key_prop k == p}
 
-
 assume val leak: k:key { forall t. key_prop k t } -> bytes 
 assume val leaked: k:key -> b:bool { b ==> (forall t. key_prop k t) }   
-// TODO why do I need parentheses?
 
 (* this function returns the key bytes, and marks the key as corrupted *)
-
-(* TODO make keys abstract except within this module *) 
 
 assume val keygen: p:(text -> Type) -> pkey p
 
@@ -65,22 +61,13 @@ val verify: k:key -> t:text -> tag -> b:bool{b ==> key_prop k t}
 
 (* the ideal implementation below uses a global log *)
 
-(* TODO Can we use a constructor instead of an attached property? *)
-(* TODO make keys abstract except within this module *) 
-
-(* TODO provide a concrete implementation of keygen, aka sample 16
-   random bytes + maybe a counter it would be better to avoid assuming
-   key_prop; see also encrypt.fst *)
-
 type entry = 
   | Entry : k:key
          -> t:text{key_prop k t}
          -> m:tag
          -> entry
 
-(* TODO why assumed? we miss toplevel side effects... *) 
-
-assume val log : ref (list entry)
+let log = ST.alloc (list entry) [] 
 
 let mac k t = 
   let m = sha1 k t in
@@ -101,10 +88,3 @@ let verify k text tag =
 //if verified && not (found || leaked k) then win:= Some(k,text,tag);
 //verified 
 
-(* VARIANT CTXT vs CPA: is the tag authenticated? 
-   otherwise do not include m:tag in the entry *)
-
-  let found    = is_Some(List.find (function (Entry k' text' tag') -> k=k' && text=text' (*CTXT: && tag=tag' *) ) !log) in 
-//verified           (* concrete: we never read the log *) 
-  verified && (found || leaked k ) (* ideal: we correct errors. *)
-//(if verified && not (found || leaked k) then winner:= Some(k,text,tag)) verified (* winning condition against for INT-CPA *)
